Todos los laboratorios terminados

Dalmau-Challenge-2.dfy
@@ -1,9 +1,6 @@
-predicate isCroissant(a:seq<int>)
+predicate method isCroissant(a:seq<int>)
 {
-    if |a| <= 1 then 
-        true 
-    else 
-        forall i :: 1 <= i < |a| ==> a[i-1] <= a[i]
+    forall i,j :: 1 <= i <= j < |a| ==> a[i] <= a[j]
 }
 
 predicate maxLength(a:seq<int>, k:int)
@@ -16,16 +13,12 @@ predicate maxLength(a:seq<int>, k:int)
         if |a| == k then
             isCroissant(a)
         else
-            assert |a| >= 2;
-            exists i :: (1 <= i < (|a|-2) ==> maxLength(a[..i] + a[(i+1)..], k))
+            exists i :: (0 <= i < |a| ==> maxLength(a[..i] + a[(i+1)..], k))
 }
 
-
-// The final value of k, represents the answer we are looking for, i.e.  we seek to stablish the relation
-// k = the maximum length upsecuence contained in a[0],...,a[N-1] (Postcondition) . EWD697 - 5
 method lengthLongestUpsecuence(a:seq<int>) returns (k:int)
     requires |a| > 0
-    ensures k >= 1 &&  maxLength(a,k) == true
+    ensures 1 <= k <= |a| &&  maxLength(a,k) == true
 {
     k := 1;             // Max upsecuence length
     var n := 1;         // Elements evaluated 
@@ -36,58 +29,48 @@ method lengthLongestUpsecuence(a:seq<int>) returns (k:int)
         // k = the maximum upsecuence contained in a[0],...,a[n-1] and 1 <= n <= N
         invariant 1 <= k <= n <= |a|
         invariant |m| == k
-        invariant maxLength(a[..n],k) == true
+        invariant maxLength(a[..n],k) == true // k is the longest upsecuence
+        invariant isCroissant(m)
         decreases |a| - n
     {
 
         if m[k-1] <= a[n] {
             k := k + 1;            // k increases as we found an upsecuence of this length
             m := m + [a[n]];       // a[n] becomes the minimum righ-most element of the upsecuence of length k containe in a[0]...a[n]
-        }else{
 
-            // We find m[j] the minimum rightmost element of an upsecuente of length j where 1 < j < k
-            if a[n] < m[0] { // New smallest beginning of subsecuence
-                m := m[0 := a[n]]; 
-            }else{
-                var i := k - 1;
-
-                while i > 0
-                    invariant 0 <= i <= k - 1  // we already know here m[k-1] is greater than a[n], no need to reach
-                {
-                    if  a[n] < m[i] {
-                        i := i - 1;
-                    } else {
-                        m := m[i := a[n]];
-                        i := 0;
-                    }
-                }
-            }
+        }else if a[n] < m[0] { // New smallest beginning of subsecuence
+            m := m[0 := a[n]]; 
+        
+        } else {   // We find m[j] the minimum rightmost element of an upsecuente of length j+1 where 0 <= j < k, in a[..n-1]
+            m := BinaryInsertion(m, a[n]);
         }
-        assume |m|== k; // TODO
+
         n := n + 1;
     }
 }
+ 
 
 // We find m[j] the minimum rightmost element of an upsecuente of length 
-// P2: forall j : 1 < j < k: m[j] = the minimum rightmost element of an upsecuence contained in A[0] .. A[n-1]
-method binarySearch(m:seq<int>, aN: int, k:int) returns (j:int)
-    requires k > 1 && |m| == k
-    requires m[0] <= aN < m[k-1] // 
-    ensures 1 < j < k-1 && m[j-1] <= aN < m[j]
-    {
-        var i,h := 0,0; // Cut point
-        j := k-1;
-        while j - i > 0
-            // P3 invaraint in Dijktras article
-            invariant 0 <= i <= j < k &&  m[i] <= aN < m[j]
-            decreases  j - i 
-            {
-                assert i != j;
-                h := (i + j)/2;
-                if m[h] <= aN {
-                    i := h;
-                }else{
-                    j := h;
-                }
-            }
-    }
+// P2: forall j : 1  < j < k: m[j] = the minimum rightmost element of an upsecuence contained in A[0] .. A[n-1]
+method BinaryInsertion(s:seq<int>, v:int) returns (s':seq<int>)
+    requires isCroissant(s)
+    requires |s| > 0
+    requires s[0] <= v < s[|s|-1]
+    ensures isCroissant(s') && v in s'
+    ensures |s| == |s'|
+    //     var start, end := 0, |a|;
+    //     while start < end
+    //     invariant 0 <= start <= end <=
+    //     invariant a[start] <= m' < a[end..]
+    //     {
+    //         var mid := (start + end) / 2;
+
+    //         if m' < a[mid] {
+    //             end := mid;
+    //         } else {
+    //             start := mid + 1;
+    //         }
+    //     }
+
+    //     b := a[mid := m'];
+    // }
