Lab5.dfy
@@ -1,31 +1,266 @@
-
 datatype List<T> = Empty | Cons(head:T, tail:List)
 
-function length<T>(xs:List<T>):int
-    decreases xs
+function length<T>(xs:List<T>):nat
 {
-    if xs.Empty? then 0 else 1 + length(xs.tail)
+//if xs.Empty? then 0 else 1+length(xs.tail)
+match xs
+	case Empty => 0
+	case Cons(_,t) => 1 + length(t)
+}
+
+function EqPairs<T(==)>(xs:List):nat
+{
+match xs
+	case Empty => 0
+	case Cons(h1,Empty) => 0
+	case Cons(h1,Cons(h2,t)) 
+	    => if h1 == h2 then 1 + EqPairs(Cons(h2,t))
+		               else EqPairs(Cons(h2,t))
 }
 
 
 datatype Tree<T> = Empty | Node(left:Tree,root:T,right:Tree)
 
-function depth<T>(t:Tree):int
-    decreases  t
+function max(x:int,y:int):int
 {
-    if t.Empty? then 0 else 1 + max(depth(t.left),depth(t.right))
+if x >= y then x else y
 }
 
-function depth2<T>(t:Tree):int
-    decreases  t
+function depth<T>(t:Tree<T>):nat
 {
-    match t {
-        case Empty => 0
-        case Node (l,_,r) =>  1 + max(depth(t.left),depth(t.right))
+//if t.Empty? then 0 else 1 + max(depth(t.left),depth(t.right))
+match t
+	case Empty => 0
+	case Node(l,_,r) => 1 + max(depth(l),depth(r))
+}
+
+predicate full<T>(t:Tree)
+{
+/*
+match t
+	case Empty => true
+	case Node(l,_,r) 
+	     => (l.Empty? && r.Empty?) ||
+		    (l.Node? && r.Node? && full(l) && full(r))
+			//!l.Empty? && !r.Empty
+*/
+t.Empty? || (t.left.Empty? && t.right.Empty?) ||
+(t.left.Node? && t.right.Node? && full(t.left) && full(t.right))
+}
+
+lemma {:induction false} EqPairs_Lemma<T(==)>(xs:List)
+	ensures EqPairs(xs) <= length(xs)
+{
+match xs {
+	case Empty => {}
+	case Cons(_,t) 
+	     => { calc {
+		            EqPairs(xs);
+					<=
+					1 + EqPairs(t);
+		            <= { EqPairs_Lemma(t);}
+					1+ length(t);
+				    ==
+					length(xs);
+				   } 
+		    }
+	}
+}
+
+function append<T>(xs:List, ys:List):List
+{
+if xs.Empty? then ys else Cons(xs.head,append(xs.tail,ys))
+}
+
+//Ejercicio: length(append(xs,ys)) == length(append(xs)) + length(append(ys))
+
+function rev<T>(xs:List):List
+{
+if xs.Empty? then List.Empty 
+             else append(rev(xs.tail),Cons(xs.head,List.Empty))
+}
+
+lemma rev_twice_Lemma<T>(xs:List)
+	ensures rev(rev(xs)) == xs
+{
+match xs 
+	case Empty => {}
+	case Cons(h,t) 
+	   => {
+           calc {
+		        rev(rev(Cons(h,t)));
+				rev(append(rev(t),Cons(h,List.Empty)));
+				== {
+				   appendDist_Lemma(rev(t),Cons(h,List.Empty));
+				   //assume forall xs:List<T>, ys :: 
+				   //rev(append(xs,ys)) == append(rev(ys),rev(xs));                  
+				   }
+				append(rev(Cons(h,List.Empty)),rev(rev(t)));
+				== { rev_twice_Lemma(t); //H.I.
+					 // assert rev(rev(t)) == t 
+					}
+			   append(Cons(h,List.Empty),t);
+			   Cons(h,t);
+	       }}
+
+}
+
+lemma appendDist_Lemma<T>(xs:List,ys:List)
+  ensures rev(append(xs,ys)) == append(rev(ys),rev(xs));
+{
+match xs 
+	case Empty => {
+	               appendEmpty_Lemma(rev(ys));
+				   //assert rev(ys) == append(rev(ys),List.Empty);
+	               }
+	case Cons(h,t) 
+	  => {
+	      calc { 
+		        rev(append(Cons(h,t),ys)); 
+		        rev(Cons(h,append(t,ys)));
+				append(rev(append(t,ys)),Cons(h,List.Empty));           
+			         == { appendDist_Lemma(t,ys);	//H.I.	   
+		                  // rev(append(t,ys)) == append(rev(ys),rev(t));
+						}
+		        append(append(rev(ys),rev(t)),Cons(h,List.Empty));
+				    == {
+					   appendAss(rev(ys),rev(t),Cons(h,List.Empty));
+					   //assert forall xs:List<T>, ys, zs :: append(append(xs,ys),zs) == append(xs,append(ys,zs));
+					   }
+				append(rev(ys), append(rev(t),Cons(h,List.Empty)));
+
+				append(rev(ys),rev(Cons(h,t)));
+		       }
+	     }
+}
+
+lemma appendAss<T>(xs:List, ys:List, zs:List)
+ ensures append(append(xs,ys),zs) == append(xs,append(ys,zs));
+{}
+
+lemma appendEmpty_Lemma<T>(xs:List)
+   ensures append(xs,List.Empty) == xs
+{}
+
+lemma appendEmptyForall_Lemma<T>()
+   ensures forall xs:List<T> :: append(xs,List.Empty) == xs
+{
+forall xs:List<T> { appendEmpty_Lemma(xs); }
+}
+
+predicate perfect<T>(t:Tree)
+{
+match t
+   case Empty => false
+   case Node(l,d,r) => (l.Empty? && r.Empty?) ||
+                       ( !l.Empty? && !r.Empty?
+					     && perfect(l) && perfect(r)
+						 && depth(l) == depth(r) )
+}
+
+function numLeaves<T>(t:Tree):nat
+{
+match t
+   case Empty => 0
+   case Node(l,d,r) => if l.Empty? && r.Empty?
+                       then 1
+					   else numLeaves(l) + numLeaves(r)
+}
+
+function exp2(n:nat):nat
+{
+if n == 0 then 1 else 2 * exp2(n-1)
+}
+
+lemma {:induction false} leavesPerfect_Lemma<T>(t:Tree)
+	requires perfect(t)
+	ensures numLeaves(t) == exp2(depth(t)-1)
+{
+match t
+  //case Empty => {}
+  case Node(l,d,r) => 
+      {
+	  calc { 
+	       numLeaves(Node(l,d,r));
+		   if l.Empty? && r.Empty? then 1 
+		   else numLeaves(l) + numLeaves(r);
+		   == { 
+		       if perfect(l) { leavesPerfect_Lemma(l);}
+			   if perfect(r) { leavesPerfect_Lemma(r);}
+	           // numLeaves(l) == exp2(depth(l)-1)
+	           // numLeaves(r) == exp2(depth(r)-1)
+			   }
+		   if l.Empty? && r.Empty? then 1 
+		   else exp2(depth(l)-1) + exp2(depth(r)-1);
+
+		   if l.Empty? && r.Empty? then 1  else 2 * exp2(depth(l)-1);
+
+		   if l.Empty? && r.Empty? then 1  else exp2(depth(l));
+
+	       exp2(depth(t)-1);
+		   }
+	  }
+}
+
+function numNodes<T>(t:Tree):nat
+{
+match t
+   case Empty => 0
+   case Node(l,d,r) => 1 + numNodes(l) + numNodes(r)
+}
+
+lemma nodesPerfect_Lemma<T>(t:Tree)
+	requires perfect(t)
+	ensures numNodes(t) == exp2(depth(t)) - 1
+// Ejercicio
+
+function mirror<T>(t:Tree):Tree
+{
+match t
+	case Empty => Tree.Empty
+	case Node(l,d,r) => Node(mirror(r),d,mirror(l))
+}
+
+lemma {:induction false} mirrorTwice_Lemma<T>(t:Tree)
+	ensures mirror(mirror(t)) == t
+{
+match t 
+	case Empty => {}
+	case Node(l,d,r) => {
+	                     calc {
+						       mirror(mirror(t)); 
+							   mirror(Node(mirror(r),d,mirror(l)));
+							   Node(mirror(mirror(l)),d,mirror(mirror(r)));
+							    == {
+								    mirrorTwice_Lemma(l); 
+									mirrorTwice_Lemma(r);
+								   }
+							   Node(l,d,r);
+						 }
+	                    } 
+	                   
+}
+
+function multiset_of_tree<T>(t:Tree): multiset<T>
+{
+match t
+	case Empty => multiset{}
+	case Node(l,x,r) => multiset{x} + multiset_of_tree(l)
+	                                + multiset_of_tree(r)
+}
+
+lemma {:induction false} multisetTree_Lemma<T>(t:Tree)
+	ensures multiset_of_tree(mirror(t)) == multiset_of_tree(t)
+    {
+        match t 
+            case Empty => {}
+            case Node(l,d,r) => {
+                                calc {
+                                        multiset_of_tree(mirror(t));
+                                        {multisetTree_Lemma(l);multisetTree_Lemma(r);}
+                                        multiset_of_tree(t);
+                                    }
+                                } 
+	                   
     }
-}
-
-function max(a:int, b:int):int
-{
-    if a < b then b else a
-}
+// Ejercicio 
