5-Ass-Dalmau.dfy
@@ -1,0 +1,172 @@
+datatype List<T> = Nil | Cons(head:T, tail:List<T>)
+
+datatype Tree<T> = Empty | Node(left:Tree,data:T,right:Tree)
+
+function length (xs:List):nat
+{
+match xs
+	case Nil => 0
+	case Cons(_,t) => 1 + length(t)
+}
+
+function multiset_of_list<T> (xs:List<T>): multiset<T>
+{
+match xs
+	case Nil => multiset{}
+	case Cons(h,t) => multiset{h} + multiset_of_list(t)
+}
+
+function append<T> (xs:List, ys:List): List 
+{
+match xs
+    case Nil => ys
+    case Cons(h,t) => Cons(h,append(t,ys))
+}
+
+function mirror (t:Tree):Tree
+{
+match t
+	case Empty => Empty
+	case Node(l,d,r) => Node(mirror(r),d,mirror(l))
+}
+
+function flatten<T> (t:Tree):List<T>
+{
+match t
+	case Empty => Nil
+	case Node(l,d,r) => append(flatten(l), Cons(d,flatten(r)))
+}
+
+// Exercise 1
+// Prove this lemma
+lemma {:induction false} Lemma_mirror_multiset (t:Tree)
+	ensures multiset_of_list(flatten(t)) == multiset_of_list(flatten(mirror(t)))
+    {
+         match t 
+            case Empty => {}
+            case Node(l,d,r) => {
+                                calc {
+                                        multiset_of_list(flatten(t));
+                                        {multisetOfTree_Lemma(t);}
+                                        multiset_of_list(flatten(l)) + multiset{d} + multiset_of_list(flatten(r));
+                                        {
+                                            Lemma_mirror_multiset(l);
+                                            Lemma_mirror_multiset(r);
+                                        }
+                                        multiset_of_list(flatten(mirror(l))) + multiset{d} +  multiset_of_list(flatten(mirror(r)));
+                                        {multisetOfTree_Lemma(Node(mirror(r),d,mirror(l)));}
+                                        multiset_of_list(flatten(Node(mirror(r),d,mirror(l))));
+                                    }
+                                } 
+    }
+
+lemma multisetOfListAppend_Lemma(l:List, r:List)
+    ensures multiset_of_list(append(l,r)) == multiset_of_list(l) + multiset_of_list(r);
+    {}
+
+lemma multisetOfTree_Lemma(t:Tree)
+    requires t.Node?
+    ensures multiset_of_list(flatten(t)) == multiset_of_list(flatten(t.left)) + multiset{t.data} +  multiset_of_list(flatten(t.right));
+    {
+        calc{
+            multiset_of_list(flatten(t));
+            multiset_of_list(append(flatten(t.left), Cons(t.data,flatten(t.right))));
+            {multisetOfListAppend_Lemma(flatten(t.left), Cons(t.data,flatten(t.right)));}
+            multiset_of_list(flatten(t.left)) + multiset{t.data} +  multiset_of_list(flatten(t.right));   
+        }
+    }
+
+// Exercise 2
+
+function numLeaves(t:Tree):nat
+{
+match t
+	case Empty => 0
+	case Node(l,d,r) => if l.Empty? && r.Empty? then 1
+	                    else numLeaves(l) + numLeaves(r)
+}
+
+// Define a function that calculates the number of nodes of degree 2 of a given tree.
+// A node has grade 2 if it has exactly two children
+// Complete the definition
+function numDegree2 (t:Tree):nat
+{
+    match t
+        case Empty => 0
+        case Node(l,d,r) =>
+            if l.Empty? || r.Empty? then 
+                numDegree2(r) + numDegree2(l)
+            else 
+                1 + numDegree2(r) + numDegree2(l)
+}
+
+// Prove this lemma
+lemma {:induction false} Degree2_Lemma (t:Tree)
+	requires t.Node?
+	ensures numLeaves(t) == numDegree2(t)+1
+    {  
+        match t
+            case Node(l,d,r) => {
+                calc {
+                    numLeaves(t);
+                    if l.Empty? && r.Empty? then 1 else numLeaves(l) + numLeaves(r);
+                    {
+                        if l.Node? {Degree2_Lemma(l);}
+                        if r.Node? {Degree2_Lemma(r);}    
+                    }
+                    // El siguiente bloque no es obligatorio, el SMT solver lo comprueba
+                    if l.Empty? || r.Empty? then 
+                        numDegree2(r) + numDegree2(l) + 1
+                    else 
+                        numDegree2(r) + 1 + numDegree2(l) + 1;
+                    numDegree2(t)+1;
+                }
+            }
+    }
+
+// Exercise 3
+
+predicate method isLeaf<T> (t:Tree)            // Note that it can be used in code   
+{
+t.Node? && t.left.Empty? && t.right.Empty? 
+}
+
+function Leaves<T> (t:Tree):set<T>
+{
+match t
+	case Empty => {}
+	case Node(l,d,r) => if l.Empty? && r.Empty? then {d}
+	                    else Leaves(l) + Leaves(r)
+}
+
+method MaxLeave (t:Tree<nat>) returns (max:nat)
+    requires t.Node?
+	ensures max in Leaves(t) 
+	ensures forall d :: d in Leaves(t) ==> d <= max
+{   
+    var maxL, maxR := 0,0;
+    if isLeaf(t) {
+        max := t.data;
+    }else {
+        if !t.left.Empty? { 
+            maxL := MaxLeave(t.left);
+        }
+        if !t.right.Empty? {
+            maxR := MaxLeave(t.right);
+        }
+        if maxL < maxR {
+            max := maxR;
+        } else {
+            max := maxL;
+        }
+    }
+}
+// Design a verified body for that method.
+// As a hint you can use the following assert that can be preoviously checked to be true.
+
+/*
+assert t.Node? ==> Leaves(t) == if isLeaf(t) then {t.data} 
+                                else ((if !t.left.Empty? then Leaves(t.left) else {})
+								      + (if !t.right.Empty? then Leaves(t.right) else {}));
+*/
+               
